Iterator/HetT.lean
@@ -14,7 +14,7 @@ arbitrary universes.
 There's a caveat to saying "efficiently":
 * The base monad is bundled together with a `Prop` and a proof. The latter two are erased at runtime
   as far as I can tell. However, Since this monad is not a function type but a structure,
-  it should only be used in functions that are inlined.
+  it should only be used in functions that are inlined, especially not in recursive ones.
 * We occasionally need to insert `map` applications where the function will be compiled to the identity.
   Unfortunately, these currently aren't always optimized away, see the example below with the IO monad.
 -/
@@ -28,12 +28,27 @@ structure HetT (m : Type w → Type w') (α : Type u) where
 instance (m : Type w → Type w') [Functor m] : MonadLift m (HetT m) where
   monadLift x := ⟨fun _ => True, inferInstance, (fun x => .deflate ⟨x, True.intro⟩) <$> x⟩
 
+def HetT.liftSquashed {m : Type w → Type w'} {α : Type u} [Functor m] [Small.{w} α] (x : m (USquash α)) :
+    HetT m α :=
+  ⟨fun _ => True, sorry, (fun x => .deflate ⟨x.inflate, True.intro⟩) <$> x⟩
+
+@[always_inline, inline]
+protected def HetT.mapH {m : Type w → Type w'} [Functor m] {α : Type u} {β : Type v}
+    (f : α → β) (x : HetT m α) : HetT m β :=
+  ⟨fun b => ∃ a : Subtype x.property, f a.1 = b, sorry,
+    (fun a => .deflate ⟨f (a.inflate (small := _)).val, _, rfl⟩ (small := _)) <$> x.computation⟩
+
 @[always_inline, inline]
 protected def HetT.bindH {m : Type w → Type w'} [Monad m] {α : Type u} {β : Type v} (x : HetT m α) (f : α → HetT m β) : HetT m β :=
-    ⟨fun b => ∃ a, x.property a ∧ (f a).property b, sorry,
-      x.computation >>= fun a => letI a := a.inflate (small := _);
-        (fun b => letI b := b.inflate (small := _);
-          .deflate (small := _) <| ⟨b.val, a.val, a.property, b.property⟩) <$> (f a).computation⟩
+  ⟨fun b => ∃ a, x.property a ∧ (f a).property b, sorry,
+    x.computation >>= fun a => letI a := a.inflate (small := _);
+      (fun b => letI b := b.inflate (small := _);
+        .deflate (small := _) <| ⟨b.val, a.val, a.property, b.property⟩) <$> (f a).computation⟩
+
+@[always_inline, inline]
+protected def HetT.liftMapH {m : Type w → Type w'} [Monad m] {α : Type w} {β : Type v}
+    (f : α → β) (x : m α) : HetT m β :=
+  ⟨fun b => ∃ a, f a = b, sorry, (fun a => .deflate ⟨f a, a, rfl⟩ (small := _)) <$> x⟩
 
 @[always_inline, inline]
 def HetT.run {m : Type w → Type w'} [Monad m] {α : Type w} (x : HetT m α) : m α :=
@@ -42,6 +57,23 @@ def HetT.run {m : Type w → Type w'} [Monad m] {α : Type w} (x : HetT m α) : 
 instance {m : Type w → Type w'} [Monad m] : Monad (HetT.{w, w', u} m) where
   pure x := ⟨fun y => x = y, sorry, pure <| .deflate (small := _) ⟨x, rfl⟩⟩
   bind x f := x.bindH f
+
+@[simp]
+theorem HetT.property_mapH {m : Type w → Type w'} [Functor m] {α : Type u} {β : Type v}
+    {x : HetT m α} {f : α → β} {b : β} :
+    (x.mapH f).property b ↔ (∃ a, f a = b ∧ x.property a) := by
+  simp only [HetT.mapH]
+  apply Iff.intro
+  · rintro ⟨⟨a, ha⟩, h⟩
+    exact ⟨a, h, ha⟩
+  · rintro ⟨a, h, ha⟩
+    exact ⟨⟨a, ha⟩, h⟩
+
+@[simp]
+theorem HetT.computation_mapH {m : Type w → Type w'} [Functor m] {α : Type u} {β : Type v}
+    {x : HetT m α} {f : α → β} {b : β} :
+    (x.mapH f).computation = (fun a => .deflate ⟨_, a.inflate (small := _), rfl⟩ (small := _)) <$> x.computation :=
+  rfl
 
 set_option trace.compiler.ir.result true in
 def test : IO Unit := do
