Iterator/Consumers/Loop.lean
@@ -1,12 +1,12 @@
-import Iterator.Wrapper
+import Iterator.Basic
 
-class IteratorFor (α : Type u) (m : Type w → Type w') (β : Type v) [Iterator α m β] (n : Type w → Type w'') where
+class IteratorFor (α : Type w) (m : Type w → Type w') (β : Type v) [Iterator α m β] (n : Type w → Type w'') where
   forIn : ∀ {γ : Type w}, Iter (α := α) m β → γ → (β → γ → n (ForInStep γ)) → n γ
 
 @[specialize]
 def Iter.DefaultConsumers.forIn {m : Type w → Type w'} {n : Type w → Type w''} [Monad m] [Monad n] [MonadLiftT m n]
-    {α : Type u} {β : Type v} {γ : Type w}
-    {_ : Iterator α m β} [Finite α m]
+    {α : Type w} {β : Type v} {γ : Type w}
+    [Iterator α m β] [Finite α m]
     (it : Iter (α := α) m β) (init : γ) (f : β → γ → n (ForInStep γ)) : n γ := do
   match (← it.stepH).inflate with
   | .yield it' out _ =>
@@ -15,16 +15,16 @@ def Iter.DefaultConsumers.forIn {m : Type w → Type w'} {n : Type w → Type w'
     | .done c => return c
   | .skip it' _ => Iter.DefaultConsumers.forIn it' init f
   | .done _ => return init
-termination_by it.terminationByFinite
+termination_by it.finitelyManySteps
 
 instance {m : Type w → Type w'} {n : Type w → Type w''} [Monad m]
-    {α : Type u} {β : Type v} {_ : Iterator α m β} [IteratorFor α m β n] :
+    {α : Type w} {β : Type v} [Iterator α m β] [IteratorFor α m β n] :
     ForIn n (Iter (α := α) m β) β where
   forIn := IteratorFor.forIn
 
 @[specialize]
 def Iter.foldM {m : Type w → Type w'} {n : Type w → Type w'} [Monad m] [Functor n]
-    {α : Type u} {β : Type v} {γ : Type w} {_ : Iterator α m β} [IteratorFor α m β n]
+    {α : Type w} {β : Type v} {γ : Type w} [Iterator α m β] [IteratorFor α m β n]
     (f : γ → β → n γ) (init : γ) (it : Iter (α := α) m β) : n γ :=
   IteratorFor.forIn it init (fun x acc => ForInStep.yield <$> f acc x)
 
@@ -38,10 +38,10 @@ where
     | .yield it' _ _ => go it' (acc + 1)
     | .skip it' _ => go it' acc
     | .done _ => acc
-  termination_by it.terminationByFinite
+  termination_by it.finitelyManySteps
 
 @[specialize]
-def Iter.countM {m : Type → Type w'} [Monad m] {α : Type u} {β : Type v} {_ : Iterator α m β} [Finite α m] {_ : ComputableSmall.{0} α}
+def Iter.countM {m : Type → Type w'} [Monad m] {α : Type} {β : Type v} [Iterator α m β] [Finite α m] {_ : ComputableSmall.{0} α}
     (it : Iter (α := α) m β) : m Nat :=
   go it 0
 where
@@ -50,10 +50,10 @@ where
       | .yield it' _ _ => go it' (acc + 1)
       | .skip it' _ => go it' acc
       | .done _ => return acc
-  termination_by it.terminationByFinite
+  termination_by it.finitelyManySteps
 
 @[specialize]
-def Iter.drain {α : Type u} {m : Type w → Type w'} {β : Type v} [Monad m]
-    {_ : Iterator α m β} (it : Iter (α := α) m β) [IteratorFor α m β m] :
+def Iter.drain {α : Type w} {m : Type w → Type w'} {β : Type v} [Monad m]
+    [Iterator α m β] (it : Iter (α := α) m β) [IteratorFor α m β m] :
     m PUnit := do
   it.foldM (γ := PUnit) (fun _ _ => pure .unit) .unit
