Iterator/Consumers/Size.lean
@@ -1,4 +1,4 @@
-import Iterator.Wrapper
+import Iterator.Basic
 
 class IteratorSized (α : Type u) (m : Type w → Type w') where
   size : α → Option Nat
