Iterator/Producers.lean
@@ -9,57 +9,31 @@ import Init.Data.Nat.Lemmas
 
 section ListIterator
 
-variable {α : Type u} {m : Type w → Type w'}
+variable {α : Type w} {m : Type w → Type w'}
 
 structure ListIterator (α : Type u) where
   list : List α
-
--- instance {α} : Iterator (ListIterator α) m α where
---   step it :=
---     (fun
---       | [] => .done
---       | x :: xs => .yield { list := xs } x) <$>
---     (pure it.list : IterationT m _)
-
--- /--
--- Returns a finite iterator for the given list.
--- The iterator yields the elements of the list in order and then terminates.
--- -/
--- @[always_inline, inline]
--- def List.iter {α : Type u} (l : List α) (m : Type u → Type w := by exact Id) [ComputableSmall.{w} α] :
---     Iter (α := ListIterator α) m α :=
---   toIter m { list := l }
-
--- instance : FinitenessRelation (ListIterator α) m where
---   rel := InvImage WellFoundedRelation.rel ListIterator.list
---   wf := InvImage.wf _ WellFoundedRelation.wf
---   subrelation {it it'} h := by
---     simp_wf
---     simp only [Iterator.step, IterationT.map_eq_mapH, IterationT.mapH, Pure.pure] at h
---     obtain ⟨step, h, _, rfl, rfl⟩ := h
---     cases it
---     split at h <;> simp_all [IterStep.successor]
 
 /--
 Returns a finite iterator for the given list.
 The iterator yields the elements of the list in order and then terminates.
 -/
 @[always_inline, inline]
-def List.iter {α : Type u} (l : List α) (m : Type u → Type w := by exact Id) [Pure m] :
+def List.iter {α : Type w} (l : List α) (m : Type w → Type w' := by exact Id) [Pure m] :
     Iter (α := ListIterator α) m α :=
   toIter { list := l } m α
 
-instance {α : Type u} [Pure m] [UnivLE.{u, w}] : Iterator (ListIterator α) m α where
-  value_small := inferInstance
+instance {α : Type w} [Pure m] : Iterator (ListIterator α) m α where
   plausible_step it
     | .yield it' out => it.inner.list = out :: it'.inner.list
     | .skip _ => False
     | .done => it.inner.list = []
-  step it := letI l := it.inner; pure (match h : l with
-        | ⟨[]⟩ => .deflate ⟨.done, by simp_all [l]⟩
-        | ⟨x :: xs⟩ => .deflate ⟨.yield (toIter ⟨xs⟩ m α) x, (by simp_all [l])⟩)
+  step_small := inferInstance
+  step it := pure (match it with
+        | ⟨⟨[]⟩⟩ => .deflate ⟨.done, rfl⟩
+        | ⟨⟨x :: xs⟩⟩ => .deflate ⟨.yield (toIter ⟨xs⟩ m α) x, rfl⟩)
 
-instance [Pure m] [UnivLE.{u, w}] : FinitenessRelation (ListIterator α) m where
+instance [Pure m] : FinitenessRelation (ListIterator α) m where
   rel := InvImage WellFoundedRelation.rel (ListIterator.list ∘ Iter.inner)
   wf := InvImage.wf _ WellFoundedRelation.wf
   subrelation {it it'} h := by
@@ -73,17 +47,17 @@ section Unfold
 
 universe u v
 
-variable {α : Type u} {m : Type w → Type w'} {f : α → α}
+variable {α : Type w} {m : Type w → Type w'} {f : α → α}
 
 structure UnfoldIterator (α : Type u) (f : α → α) where
   next : α
 
-instance [Pure m] [UnivLE.{u, w}] : Iterator (UnfoldIterator α f) m α where
-  value_small := inferInstance
+instance [Pure m] : Iterator (UnfoldIterator α f) m α where
   plausible_step it
     | .yield it' out => out = it.inner.next ∧ it' = toIter ⟨f it.inner.next⟩ m α
     | .skip _ => False
     | .done => False
+  step_small := inferInstance
   step it := pure <| .deflate <| .yield (toIter ⟨f it.inner.next⟩ m α) it.inner.next (by simp)
 
 /--
@@ -91,10 +65,10 @@ Creates an infinite, productive iterator. First it yields `init`.
 If the last step yielded `a`, the next will yield `f a`.
 -/
 @[inline]
-def Iter.unfold (m : Type u → Type w') [Pure m] {α : Type u} (init : α) (f : α → α) :=
+def Iter.unfold (m : Type w → Type w') [Pure m] {α : Type w} (init : α) (f : α → α) :=
   toIter (UnfoldIterator.mk (f := f) init) m α
 
-instance [Pure m] [UnivLE.{u, w}] : ProductivenessRelation (UnfoldIterator α f) m where
+instance [Pure m] : ProductivenessRelation (UnfoldIterator α f) m where
   rel := emptyWf.rel
   wf := emptyWf.wf
   subrelation {it it'} h := by cases h
